aequiv example proved

tutorial/Imp_Equiv.v
@@ -5,9 +5,13 @@ From ITree Require Import
      ITreeFacts
      Events.MapDefault
      StateFacts
+     StateKleisli
      Eq.
 From Coq Require Import
-     String.
+     String
+     Setoid
+     Morphisms
+     Arith.
 
 (**
    The chapter [Equiv] from _Programming Language Foundations_ introduced a
@@ -24,6 +28,8 @@ From Coq Require Import
    YZ: Not really though, depends on the interpretation obviously
  *)
 
+Definition run_state {E A} (R : Monads.stateT env (itree E) A) (st: env) : itree E (env * A) :=     R st.
+
 Definition aequiv_strong (a1 a2: aexp): Prop :=
   denote_aexp a1 ≈ denote_aexp a2.
 
@@ -31,10 +37,10 @@ Definition eval_aexp (a: aexp) :=
   @interp_imp void1 value (denote_aexp a).
 
 Definition aequiv (a1 a2: aexp): Prop :=
-  forall s, eval_aexp a1 s ≈ eval_aexp a2 s.
+  forall s, run_state (eval_aexp a1) s ≈ run_state (eval_aexp a2) s.
 
 Definition cequiv (c1 c2: com): Prop :=
-  forall s, @interp_imp void1 _ (denote_com c1) s ≈ interp_imp (denote_com c2) s.
+  forall s, run_state (@interp_imp void1 _ (denote_com c1)) s ≈ run_state (interp_imp (denote_com c2)) s.
 
 Section Examples.
 
@@ -45,6 +51,53 @@ Section Examples.
   Definition Y : string := "Y".
   Definition Z : string := "Z".
 
+  Lemma interp_imp_ret: forall {R} (v: R) (E: Type -> Type) (g : env),
+     run_state (interp_imp (Ret v)) g ≅ (Ret (g, v) : itree E (env * R)).  
+  Proof.
+    intros.
+    unfold interp_imp, interp_map, run_state.
+    rewrite interp_ret. 
+    rewrite interp_state_ret.
+    reflexivity.
+  Qed.
+
+  (** [interp_imp] commutes with [bind]. *)
+  Lemma interp_imp_bind: forall {R S E} (t: itree (ImpState +' E) R) (k: R -> itree (ImpState +' E) S) (g : env),
+      run_state (interp_imp (ITree.bind t k)) g
+    ≅ (ITree.bind (run_state (interp_imp t) g) (fun '(g',  x) => run_state (interp_imp (k x)) g')).
+  Proof.
+    intros.
+    unfold interp_imp.
+    unfold interp_map.
+    repeat rewrite interp_bind.
+    repeat rewrite interp_state_bind.
+  Admitted. 
+ 
+  
+  Instance run_state_proper {E A} : Proper (eqm ==> eq ==> eutt eq) (@run_state E A).
+  Admitted.
+
+  Instance interp_state_proper {T E F S} (h: forall T : Type, E T -> Monads.stateT S (itree F) T) : Proper (eutt eq ==> eqm) (State.interp_state h (T := T)).
+  Admitted. 
+
+  Lemma interp_imp_trigger_get_var: forall (E: Type -> Type) (x: var) (g: env),
+    run_state (interp_imp (trigger (GetVar x))) g ≈ (Ret (g, lookup_default x 0 g) : itree E (env * value)).
+  Proof.
+    intros. unfold interp_imp, interp_map. rewrite interp_trigger.
+    rewrite tau_eutt. cbn. unfold cat, Cat_Handler, Handler.cat.
+  Admitted. 
+                                                                                                     
   Theorem aequiv_example: aequiv (X - X) 0.
   Proof.
+    unfold aequiv. intros s. unfold eval_aexp. simpl.
+    rewrite interp_imp_ret.   
+    rewrite interp_imp_bind.
+    rewrite interp_imp_trigger_get_var.
+    rewrite bind_ret, interp_imp_bind, interp_imp_trigger_get_var, bind_ret, interp_imp_ret.
+    cbn. rewrite Nat.sub_diag.
+    reflexivity.
+  Qed. 
     
+    
+      
+   
